Enriching the algebra with volatile.

theories/lang/algebra/cqp.v
@@ -8,47 +8,53 @@
 Require Import stdpp.numbers.
 
 
-Declare Scope cQp_scope.
-Delimit Scope cQp_scope with cQp.
+Declare Scope cvq_scope.
+Delimit Scope cvq_scope with cvq.
 
-Record cQp : Set := mk { is_const : bool ; frac : Qp }. 
-Add Printing Constructor cQp.
-Bind Scope cQp_scope with cQp.
-(* Coercion frac : cQp >-> Qp. *)
-  
-Module cQp.
-  
-  Definition of_Qp : Qp -> cQp := mk false.
-  (* Coercion to [Qp] *)
-  
-  Definition add (a b : cQp) : cQp :=
-    match a, b with
-    | mk false q_a, mk false q_b => mk false (q_a + q_b)
-    | mk _ q_a, mk _ q_b => mk true (q_a + q_b)
-    end.
+Module CV.
 
-  Lemma eta q : q = mk (is_const q) (frac q).
+  Record t : Set := mk { is_const : bool ; is_volatile : bool ; frac : Qp }.
+  Add Printing Constructor t.
+  Bind Scope cvq_scope with t.
+  Coercion frac : t >-> Qp.
+
+  Definition add (a b : t) : t :=
+    mk (a.(is_const) || b.(is_const)) (a.(is_volatile) || b.(is_volatile))
+       (a.(frac) + b.(frac)).
+
+  Lemma eta q : q = mk (is_const q) (is_volatile q) (frac q).
   Proof. by destruct q; intros. Qed.
 
-  Lemma refl q_c q_f : mk q_c q_f = mk q_c q_f.
+  Lemma refl v c q_f : mk v c q_f = mk v c q_f.
   Proof. done. Qed.
-  
-  Module Import notations.
 
-    Notation "1" := (mk false (pos_to_Qp 1)) : cQp_scope.
-    Notation "1__const" := (mk true (pos_to_Qp 1)) : cQp_scope.
-    Infix "+" := add : cQp_scope.
+  (* Notations -- probably actually make these notations? *)
+  Definition mut : Qp -> t := mk false false.
+  Definition const : Qp -> t := mk true false.
+  Definition volatile : Qp -> t := mk false true.
+  Definition const_volatile : Qp -> t := mk true true.
 
-  End notations.
-  
-End cQp.
+  Notation c := const.
+  Notation v := volatile.
+  Notation cv := const_volatile.
+  Notation vc := const_volatile (only parsing).
+  Notation m := mut.
 
-(* TODO: which Qp's to fix into cQp and which we leave? *)
-#[global] Coercion cQp.of_Qp : Qp >-> cQp.
-  
-Export cQp.notations.
+End CV.
 
-(* 
+(* as with C++, we make mutable the default *)
+#[global] Coercion CV.mut : Qp >-> CV.t.
+
+Module Type TEST.
+  Variable TEST : CV.t -> CV.t -> CV.t -> CV.t -> Prop.
+
+  (* TODO: to make this work without the [%Qp], we need to register the
+     notations for [Qp] as notations in [cvq_scope]. *)
+  Goal TEST 1%Qp (CV.c 1) (CV.v 1) (CV.cv 1).
+  Abort.
+
+End TEST.
+(*
 #[global] Notation Qp_plain := stdpp.numbers.Qp.
 #[global] Notation Qp := cQp.
 *)
