theories/lang/cpp/logic/heap_pred.v
@@ -26,7 +26,7 @@ Section defs.
 
   (** object identity *)
   Definition identityR {σ : genv} (cls : globname) (mdc : list globname)
-             (q : cQp) : Rep :=
+             (q : CV.t) : Rep :=
     as_Rep (@identity _ _ σ cls mdc q).
   (** cpp2v-core#194: [Fractional], [AsFractional], [Timeless]? *)
   (** cpp2v-core#194: The fraction is valid? Agreement? *)
@@ -62,7 +62,7 @@ Section with_cpp.
    *
    * NOTE [ty] *must* be a primitive type.
    *)
-  Definition primR_def {resolve:genv} (ty : type) (q : cQp) (v : val) : Rep :=
+  Definition primR_def {resolve:genv} (ty : type) (q : CV.t) (v : val) : Rep :=
     as_Rep (fun addr => tptsto ty q addr v **
                       [| not(exists raw, v = Vraw raw) |] **
                       [| has_type v (drop_qualifiers ty) |]).
@@ -90,23 +90,23 @@ Section with_cpp.
     : Timeless (primR ty q v).
   Proof. rewrite primR_eq. apply _. Qed.
 
-  #[global] Instance primR_fractional resolve ty v q_c :
-    Fractional (λ q, primR ty (cqp.mk q_c q) v).
+  #[global] Instance primR_fractional resolve ty v q_v q_c :
+    Fractional (λ q, primR ty (CV.mk q_v q_c q) v).
   Proof. rewrite primR_eq. apply _. Qed.
-  #[global] Instance primR_as_fractional resolve ty q q_c v fq :
-    q = cqp.mk q_c fq ->
+  #[global] Instance primR_as_fractional resolve ty q q_v q_c v fq :
+    q = CV.mk q_v q_c fq ->
     AsFractional (primR ty q v)
-      (λ q', (fun q' => primR ty (cqp.mk q_c q') v) q') fq.
-  Proof. constructor. subst. done. apply _. Qed. 
+      (λ q', (fun q' => primR ty (CV.mk q_v q_c q') v) q') fq.
+  Proof. constructor. subst. done. apply _. Qed.
 
-  Hint Extern 100 (_  = cqp.mk _ _) => apply cQp.eta : typeclass_instances.
-  Hint Extern 100 (_  = cqp.mk _ _) => apply cQp.refl : typeclass_instances.
-  
-  #[global] Instance primR_observe_frac_valid resolve ty (q : cQp) v q_f :
-    q_f = cqp.frac q ->
+  Hint Extern 100 (_  = CV.mk _ _ _) => apply CV.eta : typeclass_instances.
+  Hint Extern 100 (_  = CV.mk _ _ _) => apply CV.refl : typeclass_instances.
+
+  #[global] Instance primR_observe_frac_valid resolve ty (q : CV.t) v q_f :
+    q_f = CV.frac q ->
     Observe [| (q_f ≤ 1)%Qp |] (primR ty q v).
   Proof. rewrite primR_eq=>->. apply _. Qed.
-  
+
   #[global] Instance primR_observe_agree resolve ty q1 q2 v1 v2 :
     Observe2 [| v1 = v2 |]
       (primR ty q1 v1)
@@ -147,7 +147,7 @@ Section with_cpp.
      TODO is it possible to generalize this to support aggregate types? structures seem easy enough
           but unions seem more difficult, possibly we can achieve that through the use of disjunction?
    *)
-  Definition uninitR_def {resolve:genv} (ty : type) (q : cQp) : Rep :=
+  Definition uninitR_def {resolve:genv} (ty : type) (q : CV.t) : Rep :=
     as_Rep (fun addr => @tptsto _ _ resolve ty q addr Vundef).
   Definition uninitR_aux : seal (@uninitR_def). Proof. by eexists. Qed.
   Definition uninitR := uninitR_aux.(unseal).
@@ -171,15 +171,15 @@ Section with_cpp.
     : Timeless (uninitR ty q).
   Proof. rewrite uninitR_eq. apply _. Qed.
 
-  #[global] Instance uninitR_fractional resolve ty c_q :
-    Fractional (fun q => uninitR ty (cqp.mk c_q q)).
+  #[global] Instance uninitR_fractional resolve ty q_v q_c :
+    Fractional (fun q => uninitR ty (CV.mk q_v q_c q)).
   Proof. rewrite uninitR_eq. apply _. Qed.
-  #[global] Instance unintR_as_fractional resolve ty c_q q :
-    AsFractional (uninitR ty (cqp.mk c_q q)) (fun q => uninitR ty (cqp.mk c_q q)) q.
+  #[global] Instance unintR_as_fractional resolve ty q_v q_c q :
+    AsFractional (uninitR ty (CV.mk q_v q_c q)) (fun q => uninitR ty (CV.mk q_v q_c q)) q.
   Proof. constructor. done. apply _. Qed.
 
-  #[global] Instance uninitR_observe_frac_valid resolve ty (q : cQp) :
-    Observe [| cqp.frac q ≤ 1 |]%Qp (uninitR ty q).
+  #[global] Instance uninitR_observe_frac_valid resolve ty (q : CV.t) :
+    Observe [| CV.frac q ≤ 1 |]%Qp (uninitR ty q).
   Proof. rewrite uninitR_eq. apply _. Qed.
 
   Lemma test:
@@ -194,9 +194,9 @@ Section with_cpp.
 
   (** This seems odd, but it's relevant to proof that [anyR] is fractional. *)
   Lemma primR_uninitR {resolve} ty c_q q1 q2 v :
-    primR ty (cqp.mk c_q q1) v |--
-    uninitR ty (cqp.mk c_q q2) -*
-    primR ty (mk c_q (q1 + q2)) Vundef.
+    primR ty (CV.mk c_q q1) v |--
+    uninitR ty (CV.mk c_q q2) -*
+    primR ty (CV.mk c_q (q1 + q2)) Vundef.
   Proof.
     rewrite primR_eq/primR_def uninitR_eq/uninitR_def. constructor=>p /=.
     rewrite monPred_at_wand. iIntros "[T1 [%Hnotraw %Hty]]" (? <-%ptr_rel_elim) "/= T2".
@@ -209,11 +209,11 @@ Section with_cpp.
 
   (** [anyR] The argument pointers points to a value of C++ type [ty] that might be
       uninitialized. *)
-  Parameter anyR : ∀ {resolve} (ty : type) (q : cQp), Rep.
+  Parameter anyR : ∀ {resolve} (ty : type) (q : CV.t), Rep.
   #[global] Arguments anyR {resolve} ty q : rename.
   Axiom anyR_timeless : ∀ resolve ty q, Timeless (anyR ty q).
   Axiom anyR_fractional : ∀ resolve ty c_q, Fractional (fun q => anyR ty (cqp.mk c_q q)).
-  Axiom anyR_observe_frac_valid : ∀ resolve ty (q : cQp),
+  Axiom anyR_observe_frac_valid : ∀ resolve ty (q : CV.t),
     Observe [| cqp.frac q ≤ 1 |]%Qp (anyR ty q).
   Axiom primR_anyR : ∀ resolve t q v, primR t q v |-- anyR t q.
   Axiom uninitR_anyR : ∀ resolve t q, uninitR t q |-- anyR t q.
@@ -372,7 +372,7 @@ Section with_cpp.
 
   (** [blockR sz q] represents [q] ownership of a contiguous chunk of
       [sz] bytes without any C++ structure on top of it. *)
-  Definition blockR_def {σ} sz (q : cQp) : Rep :=
+  Definition blockR_def {σ} sz (q : CV.t) : Rep :=
     _offsetR (o_sub σ Tu8 (Z.of_N sz)) validR **
     (* ^ Encodes valid_ptr (this .[ Tu8 ! sz]). This is
     necessary to get [l |-> blockR n -|- l |-> blockR n ** l .[ Tu8 ! m] |-> blockR 0]. *)
@@ -395,7 +395,7 @@ Section with_cpp.
     AsFractional (blockR sz (mk c_q q)) (fun q => blockR sz (cqp.mk c_q q)) q.
   Proof. exact: Build_AsFractional. Qed.
 
-  #[global] Instance blockR_observe_frac_valid resolve sz (q : cQp) :
+  #[global] Instance blockR_observe_frac_valid resolve sz (q : CV.t) :
     TCLt (0 ?= sz)%N ->
     Observe [| cqp.frac q ≤ 1 |]%Qp (blockR sz q).
   Proof.
@@ -408,7 +408,7 @@ Section with_cpp.
    * it is a convenient short-hand since it happens frequently, but there is nothing
    * special about it.
    *)
-  Definition tblockR {σ} (ty : type) (q : cQp) : Rep :=
+  Definition tblockR {σ} (ty : type) (q : CV.t) : Rep :=
     match size_of σ ty , align_of ty with
     | Some sz , Some al => blockR (σ:=σ) sz q ** alignedR al
     | _ , _  => False
